Changed symbol-< to symbol< (also changed merge-symbol-< to merge-symbol<, etc.).  Changed logical-defun to get-defun-event.  Updated *acl2-exports* for these changes and by including four symbols from constant *acl2-exports-exclusions* in community book books/misc/check-acl2-exports.lisp.  Added a link to memoize (option :INVOKE) in :DOC defattach.  Extended :doc build::cert_param and added defpointers.  Briefly documented acl2-unwind-protect in :doc system-utilities.
Quoting :doc note-8-4:

  The function symbol symbol< replaces the function symbol symbol-<.
  More generally, for every built-in function symbol and theorem name
  containing "SYMBOL-<", that string in its [symbol-name] is replaced
  by "SYMBOL<".  The function logical-defun is similarly replaced by
  get-defun-event.  Thanks to Alessandro Coglio for suggesting these
  changes.  Note that the old function names still work in ACL2
  Version 8.4, as they are macro-alias for the corresponding new
  function names (see [add-macro-alias]); however, they are
  deprecated and will probably not be supported later ACL2 versions.
  (A deprecation warning is printed each time one of those macros is
  expanded by ACL2.)

The main change to :doc build::cert_param is to extend the list of
directives to be, I hope, complete.  I also added a defpointer for
each of these, e.g., uses-glucose, pointing to :doc build::cert_param.
Thanks to Eric Smith for suggesting these improvements.  Oh, and I
deleted mention of build/certlib.pl in :doc build::cert_param since
that file seems not to exist any longer; I'm guessing that it was
replaced by books/build/lib/Certlib.pm, and I didn't see any specific
cert_param values mentioned there.

Thanks to Eric Smith as well for suggesting documentation of
acl2-unwind-protect in :doc system-utilities.

axioms.lisp
@@ -1517,7 +1517,7 @@ evaluated.  See :DOC certify-book, in particular, the discussion about ``Step
            signed-byte-p
            strip-cars
            strip-cdrs
-           symbol-<
+           symbol<
            unsigned-byte-p
            untouchable-marker
            xor
@@ -9131,7 +9131,7 @@ evaluated.  See :DOC certify-book, in particular, the discussion about ``Step
       (length str1)
     (string> str1 str2)))
 
-(defun symbol-< (x y)
+(defun symbol< (x y)
   (declare (xargs :guard (and (symbolp x) (symbolp y))))
   (let ((x1 (symbol-name x))
         (y1 (symbol-name y)))
@@ -11068,7 +11068,7 @@ evaluated.  See :DOC certify-book, in particular, the discussion about ``Step
 (defun ordered-symbol-alistp (x)
 
 ; An ordered-symbol-alist is an alist whose keys are symbols which are
-; in the symbol-< order.
+; in the symbol< order.
 
   (declare (xargs :guard t))
   (cond ((atom x) (null x))
@@ -11077,11 +11077,11 @@ evaluated.  See :DOC certify-book, in particular, the discussion about ``Step
                 (or (atom (cdr x))
                     (and (consp (cadr x))
                          (symbolp (caadr x))
-                         (symbol-< (caar x)
+                         (symbol< (caar x)
                                    (caadr x))))
                 (ordered-symbol-alistp (cdr x))))))
 
-(in-theory (disable symbol-<))
+(in-theory (disable symbol<))
 
 (defthm ordered-symbol-alistp-forward-to-symbol-alistp
   (implies (ordered-symbol-alistp x)
@@ -11095,7 +11095,7 @@ evaluated.  See :DOC certify-book, in particular, the discussion about ``Step
          (list (cons key value)))
         ((eq key (caar l))
          (cons (cons key value) (cdr l)))
-        ((symbol-< key (caar l))
+        ((symbol< key (caar l))
          (cons (cons key value) l))
         (t (cons (car l)
                  (add-pair key value (cdr l))))))
@@ -11234,7 +11234,7 @@ evaluated.  See :DOC certify-book, in particular, the discussion about ``Step
          (meter-maid 'getprops 100 symb)
          (sort (getprops1 (get symb (cdr (get world-name 'acl2-world-pair))))
                #'(lambda (x y)
-                   (symbol-< (car x) (car y)))))
+                   (symbol< (car x) (car y)))))
         ((endp world-alist)
          #+acl2-metering
          (meter-maid 'getprops 100 symb)
@@ -12537,7 +12537,7 @@ evaluated.  See :DOC certify-book, in particular, the discussion about ``Step
                                acl2::*1*-package-prefix*
                                name))
         (proposed-imports ; avoid sort-symbol-listp for toothbrush
-         (remove-adjacent-duplicates-eq (sort (copy-list imports) 'symbol-<))))
+         (remove-adjacent-duplicates-eq (sort (copy-list imports) 'symbol<))))
     (assert pkg) ; see defpkg-raw
 
 ; We bind proposed-imports to the value of the imports argument.  We do not
@@ -15588,7 +15588,7 @@ evaluated.  See :DOC certify-book, in particular, the discussion about ``Step
                                                      (package-entry-name
                                                       package-entry))
                                              ans)))))
-            (sort ans (function symbol-<))))))
+            (sort ans (function symbol<))))))
   (strip-cars (global-table state-state)))
 
 (defun global-table-cars (state-state)
@@ -16541,14 +16541,14 @@ evaluated.  See :DOC certify-book, in particular, the discussion about ``Step
             (not (string<-l x2 x1 i)))
    :hints (("Goal" :in-theory (disable member))))
 
- (defthm symbol-<-asymmetric
+ (defthm symbol<-asymmetric
    (implies (and (symbolp sym1)
                  (symbolp sym2)
-                 (symbol-< sym1 sym2))
-            (not (symbol-< sym2 sym1)))
+                 (symbol< sym1 sym2))
+            (not (symbol< sym2 sym1)))
    :hints (("Goal" :in-theory
             (set-difference-theories
-             (enable string< symbol-<)
+             (enable string< symbol<)
              '(string<-l)))))
 
  (defthm string<-l-transitive
@@ -16567,15 +16567,15 @@ evaluated.  See :DOC certify-book, in particular, the discussion about ``Step
 
  (in-theory (disable string<-l))
 
- (defthm symbol-<-transitive
-   (implies (and (symbol-< x y)
-                 (symbol-< y z)
+ (defthm symbol<-transitive
+   (implies (and (symbol< x y)
+                 (symbol< y z)
                  (symbolp x)
                  (symbolp y)
                  (symbolp z))
-            (symbol-< x z))
+            (symbol< x z))
    :rule-classes ((:rewrite :match-free :all))
-   :hints (("Goal" :in-theory (enable symbol-< string<))))
+   :hints (("Goal" :in-theory (enable symbol< string<))))
 
  (local
   (defthm equal-char-code-rewrite
@@ -16623,25 +16623,25 @@ evaluated.  See :DOC certify-book, in particular, the discussion about ``Step
              (equal (equal s1 s2) t))
     :hints (("Goal" :use symbol-equality))))
 
- (defthm symbol-<-trichotomy
+ (defthm symbol<-trichotomy
    (implies (and (symbolp x)
                  (symbolp y)
-                 (not (symbol-< x y)))
-            (iff (symbol-< y x)
+                 (not (symbol< x y)))
+            (iff (symbol< y x)
                  (not (equal x y))))
-   :hints (("Goal" :in-theory (enable symbol-< string<))))
+   :hints (("Goal" :in-theory (enable symbol< string<))))
 
  (defthm ordered-symbol-alistp-remove1-assoc-eq
    (implies (ordered-symbol-alistp l)
             (ordered-symbol-alistp (remove1-assoc-eq key l))))
 
- (defthm symbol-<-irreflexive
+ (defthm symbol<-irreflexive
    (implies (symbolp x)
-            (not (symbol-< x x)))
+            (not (symbol< x x)))
    :hints (("Goal" :use
-            ((:instance symbol-<-asymmetric
+            ((:instance symbol<-asymmetric
                         (sym1 x) (sym2 x)))
-            :in-theory (disable symbol-<-asymmetric))))
+            :in-theory (disable symbol<-asymmetric))))
 
  (defthm ordered-symbol-alistp-add-pair
    (implies (and (ordered-symbol-alistp gs)
@@ -16653,7 +16653,7 @@ evaluated.  See :DOC certify-book, in particular, the discussion about ``Step
                  (symbolp world-name)
                  (symbolp key))
             (ordered-symbol-alistp (getprops key world-name w)))
-   :hints (("Goal" :in-theory (enable symbol-<))))
+   :hints (("Goal" :in-theory (enable symbol<))))
 
  (local (defthm ordered-symbol-alistp-implies-symbol-alistp
           (implies (ordered-symbol-alistp x)
@@ -17280,12 +17280,12 @@ evaluated.  See :DOC certify-book, in particular, the discussion about ``Step
                                (t ""))))
                    (t nil))))))
 
-(defun strict-symbol-<-sortedp (x)
+(defun strict-symbol<-sortedp (x)
   (declare (xargs :guard (symbol-listp x)))
   (cond ((or (endp x) (null (cdr x)))
          t)
-        (t (and (symbol-< (car x) (cadr x))
-                (strict-symbol-<-sortedp (cdr x))))))
+        (t (and (symbol< (car x) (cadr x))
+                (strict-symbol<-sortedp (cdr x))))))
 
 (defmacro chk-ruler-extenders (x type ctx wrld)
 
@@ -17304,7 +17304,7 @@ evaluated.  See :DOC certify-book, in particular, the discussion about ``Step
          (cond (msg ,(cond ((eq type 'soft) `(er soft ctx err-str msg))
                            (t `(illegal ctx err-str (list (cons #\0 msg))))))
                ,@(and (eq type 'hard)
-                      `(((not (strict-symbol-<-sortedp x))
+                      `(((not (strict-symbol<-sortedp x))
                          (illegal ctx err-str
                                   (list (cons #\0 "it is not sorted"))))))
                (t ,(cond ((eq type 'soft) '(value t))
@@ -23721,7 +23721,7 @@ evaluated.  See :DOC certify-book, in particular, the discussion about ``Step
                                           (strip-numeric-postfix sym)))
                               ans))))
                 (sort ans (function (lambda (x y)
-                                      (symbol-< (car x) (car y)))))))
+                                      (symbol< (car x) (car y)))))))
         (list :open-output-channels
               (let (ans)
                 (do-symbols
@@ -23734,7 +23734,7 @@ evaluated.  See :DOC certify-book, in particular, the discussion about ``Step
                                      (strip-numeric-postfix sym)))
                          ans))))
                 (sort ans (function (lambda (x y)
-                                      (symbol-< (car x) (car y)))))))
+                                      (symbol< (car x) (car y)))))))
         (list :global-table (global-table-cars *the-live-state*))
         (list :t-stack
               (let (ans)
@@ -26076,13 +26076,13 @@ Lisp definition."
 
          #-acl2-loop-only
 
-;  We'd use (symbol-<= x y) if we had it.
+;  We'd use (symbol<= x y) if we had it.
 
-         (not (symbol-< y x))
+         (not (symbol< y x))
          #+acl2-loop-only
          (cond ((symbolp x)
                 (cond ((symbolp y)
-                       (not (symbol-< y x)))
+                       (not (symbol< y x)))
                       (t t)))
                ((symbolp y) nil)
                (t (bad-atom<= x y))))))
@@ -26159,7 +26159,7 @@ Lisp definition."
            (alphorder x z))
   :rule-classes ((:rewrite :match-free :all))
   :hints (("Goal"
-           :in-theory (enable string< symbol-<))))
+           :in-theory (enable string< symbol<))))
 
 (defthm alphorder-anti-symmetric
   (implies (and (not (consp x))
@@ -26169,7 +26169,7 @@ Lisp definition."
            (equal x y))
   :hints (("Goal"
            :in-theory (union-theories
-                       '(string< symbol-<)
+                       '(string< symbol<)
                        (disable code-char-char-code-is-identity))
            :use ((:instance symbol-equality (s1 x) (s2 y))
                  (:instance bad-atom<=-antisymmetric)
@@ -26190,7 +26190,7 @@ Lisp definition."
                 (not (consp y)))
            (or (alphorder x y) (alphorder y x)))
   :hints (("Goal" :use (:instance bad-atom<=-total)
-           :in-theory (enable string< symbol-<)))
+           :in-theory (enable string< symbol<)))
   :rule-classes
   ((:forward-chaining :corollary
                       (implies (and (not (alphorder x y))
