books/kestrel/utilities/my-get-event.lisp
@@ -24,8 +24,8 @@
 ;; TODO: We could consider changing DEFUNS to MUTUAL-RECURSION in the result,
 ;; but functions defined with DEFUNS seem rare.
 
-;; TDOO: Consider using logical-defun, which works for :program mode functions
-;; too (but check that the :verify-guards xarg is right).
+;; TDOO: Consider using get-defun-event, which works for :program mode
+;; functions too (but check that the :verify-guards xarg is right).
 
 (include-book "std/util/bstar" :dir :system) ;could drop even this
 
